examples/dm4free/FStar.State.fst
@@ -1,55 +1,22 @@
 module FStar.State
 
 (** We try to recover the state monad from its presentation.                 **
- ** We restrict ourself to only one cell containing an integer in order to   **
- ** keep the presentation simple.                                            **)
-
-
-
-
-(** The state monad can be given by the following presentation               **
- **                                                                          **
- ** One lookup/read operation whose arity depends on the content of the cell **
- ** (in our case the arity is \aleph_0 since we store an integer)             **
- ** For each possible cell content [n] we are giving a continuation          **
- **                                                                          **
- **    Read : (int -> state a) -> state a                                    **
- **                                                                          **
- ** A write operation for each potential element in the store                **
- **                                                                          **
- **    Write : int -> state a -> state a                                     **
- **                                                                          **
- ** There are then 3 equations relating these operations                     **
- **                                                                          **
- **   Write p (Write q cont) == Write q cont                                 **
- **   Write p (Read f) == Write p (f p)                                      **
- **   Read (fun p -> Write p cont) == cont                                   **
- **                                                                          **
- ** It can then be proved that orientating correctly these equations leads   **
- ** to a strongly normalizing and confluent rewriting system whose normal    **
- ** forms are given by                                                       **
- **                                                                          **
- **    Read (fun n -> Write (f n) (Return (g n)))                            **
- **                                                                          **
- ** This normal form means exactly that elements of [state a] are of the form**
- **                                                                          **
- **    int -> a * int                                                        **)
-
+ ** See FStar.StateInt for an explanation in the case where the state is int **)
 
 (** We first define the operations **)
-noeq type free_state (a:Type0) =
-  | Return : a -> free_state a
-  | Write : int -> free_state a -> free_state a
-  | Read : f:(int -> free_state a) -> free_state a
+noeq type free_state (s a:Type0) =
+  | Return : a -> free_state s a
+  | Write : s -> free_state s a -> free_state s a
+  | Read : f:(s -> free_state s a) -> free_state s a
 
 (** and the normal forms **)
-let is_normalized1 m =
-  Read? m /\ (forall (n:int). match Read?.f m n with | Write _ (Return _) -> True | _ -> False)
+let is_normalized1 (#s #a:Type) (m : free_state s a) =
+  Read? m /\ (forall (n:s). match Read?.f m n with | Write _ (Return _) -> True | _ -> False)
 
 let is_normalized = is_normalized1
 
 (** which allows us to carve out the subtype of state **)
-let state (a:Type) = m:(free_state a){is_normalized m}
+let state (s a:Type) = m:(free_state s a){is_normalized m}
 
 
 (** We then proceed by defining a normalization procedure  **
@@ -63,8 +30,8 @@ let apply (#a #b : Type) (f : a -> Tot b) (x: a)
 = precede_app f x ; f x
 
 (* Need to be toplevel because of #786 *)
-let rec normalize_aux (#a:Type0) (m : free_state a) (n:int)
-        : Pure (free_state a)
+let rec normalize_aux (#s #a:Type0) (m : free_state s a) (n:s)
+        : Pure (free_state s a)
                (requires True)
                (ensures (fun m -> match m with | Write _ (Return _) -> True | _ -> False))
                (decreases m)
@@ -74,28 +41,23 @@ let rec normalize_aux (#a:Type0) (m : free_state a) (n:int)
   | Write n' m' -> normalize_aux m' n'
   | Read f -> normalize_aux (apply f n) n
 
-let normalize (#a:Type0) (m : free_state a) : (m':(free_state a){is_normalized1 m'}) =
+let normalize (#s #a:Type0) (m : free_state s a) : (m':(free_state s a){is_normalized1 m'}) =
   Read (normalize_aux m)
-
-(* let is_normalized0 m = m == normalize m *)
-(* let is_normalized2 m = *)
-(*   (exists m'. {:pattern normalize m'} m == (normalize m' <: free_state _)) *)
-
 
 (** We can now define the monadic operations **)
 
-let return (#a:Type) (x:a) : state a = normalize (Return x)
-let bind (#a #b : Type) (m : state a) (f : a -> state b) : state b =
+let return (#s #a:Type) (x:a) : state s a = normalize (Return x)
+let bind (#s #a #b : Type) (m : state s a) (f : a -> state s b) : state s b =
   Read (fun n -> match Read?.f m n with
               | Write n' (Return x) -> Read?.f (f x) n')
 
 
 (** And try to show that we verify the monadic laws **)
 
-let unit_left (a b:Type) (x:a) (f : a -> state b) = assert_norm (bind (return x) f == f x)
+let unit_left (s a b:Type) (x:a) (f : a -> state s b) = assert_norm (bind (return x) f == f x)
 
 (* TODO : These two equations need some amount of functional extensionality *)
-let unit_right (a:Type) (x: state a) =
+let unit_right (s a:Type) (x: state s a) =
   admit () ; assert_norm (bind x return == x)
-let assoc (a b c : Type) (x: state a) (f : a -> state b) (g : b -> state c)
+let assoc (s a b c : Type) (x: state s a) (f : a -> state s b) (g : b -> state s c)
 = admit() ; assert (bind x (fun x0 -> bind (f x0) g) == bind (bind x f) g)
